src/MemClass.v
@@ -1,10 +1,12 @@
 Require Export Mem.
 Require Import Word.
 
+Set Universe Polymorphism.
+
 Existing Class DecEq.
 
-Instance word_dec : forall n, DecEq (word n) := weq.
-Instance nat_dec : DecEq nat := PeanoNat.Nat.eq_dec.
+Instance word_dec@{i} : forall n, DecEq@{i} (word n) := weq.
+Instance nat_dec@{i} : DecEq@{i} nat := PeanoNat.Nat.eq_dec.
 
 Module Example.
 
